Clean up anonymous binder hack.
We no longer abuse empty strings for anonymous binders. Instead, we
now have a data type for binders: a binder is either named or
anonymous.

heap_lang/lang.v
@@ -15,10 +15,14 @@ Inductive un_op : Set :=
 Inductive bin_op : Set :=
   | PlusOp | MinusOp | LeOp | LtOp | EqOp.
 
+Inductive binder := BAnom | BNamed : string → binder.
+Delimit Scope binder_scope with binder.
+Bind Scope binder_scope with expr binder.
+
 Inductive expr :=
   (* Base lambda calculus *)
   | Var (x : string)
-  | Rec (f x : string) (e : expr)
+  | Rec (f x : binder) (e : expr)
   | App (e1 e2 : expr)
   (* Base types and their operations *)
   | Lit (l : base_lit)
@@ -32,7 +36,7 @@ Inductive expr :=
   (* Sums *)
   | InjL (e : expr)
   | InjR (e : expr)
-  | Case (e0 : expr) (x1 : string) (e1 : expr) (x2 : string) (e2 : expr)
+  | Case (e0 : expr) (x1 : binder) (e1 : expr) (x2 : binder) (e2 : expr)
   (* Concurrency *)
   | Fork (e : expr)
   (* Heap *)
@@ -43,7 +47,7 @@ Inductive expr :=
   | Cas (e0 : expr) (e1 : expr) (e2 : expr).
 
 Inductive val :=
-  | RecV (f x : string) (e : expr) (* e should be closed *)
+  | RecV (f x : binder) (e : expr) (* e should be closed *)
   | LitV (l : base_lit)
   | PairV (v1 v2 : val)
   | InjLV (v : val)
@@ -55,6 +59,8 @@ Proof. solve_decision. Defined.
 Global Instance un_op_dec_eq (op1 op2 : un_op) : Decision (op1 = op2).
 Proof. solve_decision. Defined.
 Global Instance bin_op_dec_eq (op1 op2 : bin_op) : Decision (op1 = op2).
+Proof. solve_decision. Defined.
+Global Instance binder_dec_eq (x1 x2 : binder) : Decision (x1 = x2).
 Proof. solve_decision. Defined.
 Global Instance expr_dec_eq (e1 e2 : expr) : Decision (e1 = e2).
 Proof. solve_decision. Defined.
@@ -101,7 +107,7 @@ Inductive ectx_item :=
   | SndCtx
   | InjLCtx
   | InjRCtx
-  | CaseCtx (x1 : string) (e1 : expr) (x2 : string) (e2 : expr)
+  | CaseCtx (x1 : binder) (e1 : expr) (x2 : binder) (e2 : expr)
   | AllocCtx
   | LoadCtx
   | StoreLCtx (e2 : expr)
@@ -138,11 +144,12 @@ Definition fill_item (Ki : ectx_item) (e : expr) : expr :=
 Definition fill (K : ectx) (e : expr) : expr := fold_right fill_item e K.
 
 (** Substitution *)
-(** We have [subst e "" v = e] to deal with anonymous binders *)
+(** We have [subst e None v = e] to deal with anonymous binders *)
 Fixpoint subst (e : expr) (x : string) (v : val) : expr :=
   match e with
-  | Var y => if decide (x = y ∧ x ≠ "") then of_val v else Var y
-  | Rec f y e => Rec f y (if decide (x ≠ f ∧ x ≠ y) then subst e x v else e)
+  | Var y => if decide (x = y) then of_val v else Var y
+  | Rec f y e =>
+     Rec f y (if decide (BNamed x ≠ f ∧ BNamed x ≠ y) then subst e x v else e)
   | App e1 e2 => App (subst e1 x v) (subst e2 x v)
   | Lit l => Lit l
   | UnOp op e => UnOp op (subst e x v)
@@ -155,8 +162,8 @@ Fixpoint subst (e : expr) (x : string) (v : val) : expr :=
   | InjR e => InjR (subst e x v)
   | Case e0 x1 e1 x2 e2 =>
      Case (subst e0 x v)
-       x1 (if decide (x ≠ x1) then subst e1 x v else e1)
-       x2 (if decide (x ≠ x2) then subst e2 x v else e2)
+       x1 (if decide (BNamed x ≠ x1) then subst e1 x v else e1)
+       x2 (if decide (BNamed x ≠ x2) then subst e2 x v else e2)
   | Fork e => Fork (subst e x v)
   | Loc l => Loc l
   | Alloc e => Alloc (subst e x v)
@@ -164,6 +171,8 @@ Fixpoint subst (e : expr) (x : string) (v : val) : expr :=
   | Store e1 e2 => Store (subst e1 x v) (subst e2 x v)
   | Cas e0 e1 e2 => Cas (subst e0 x v) (subst e1 x v) (subst e2 x v)
   end.
+Definition subst' (e : expr) (mx : binder) (v : val) : expr :=
+  match mx with BNamed x => subst e x v | BAnom => e end.
 
 (** The stepping relation *)
 Definition un_op_eval (op : un_op) (l : base_lit) : option base_lit :=
@@ -187,7 +196,7 @@ Inductive head_step : expr → state → expr → state → option expr → Prop
   | BetaS f x e1 e2 v2 σ :
      to_val e2 = Some v2 →
      head_step (App (Rec f x e1) e2) σ
-       (subst (subst e1 f (RecV f x e1)) x v2) σ None
+       (subst' (subst' e1 f (RecV f x e1)) x v2) σ None
   | UnOpS op l l' σ :
      un_op_eval op l = Some l' → 
      head_step (UnOp op (Lit l)) σ (Lit l') σ None
@@ -206,10 +215,10 @@ Inductive head_step : expr → state → expr → state → option expr → Prop
      head_step (Snd (Pair e1 e2)) σ e2 σ None
   | CaseLS e0 v0 x1 e1 x2 e2 σ :
      to_val e0 = Some v0 →
-     head_step (Case (InjL e0) x1 e1 x2 e2) σ (subst e1 x1 v0) σ None
+     head_step (Case (InjL e0) x1 e1 x2 e2) σ (subst' e1 x1 v0) σ None
   | CaseRS e0 v0 x1 e1 x2 e2 σ :
      to_val e0 = Some v0 →
-     head_step (Case (InjR e0) x1 e1 x2 e2) σ (subst e2 x2 v0) σ None
+     head_step (Case (InjR e0) x1 e1 x2 e2) σ (subst' e2 x2 v0) σ None
   | ForkS e σ:
      head_step (Fork e) σ (Lit LitUnit) σ (Some e)
   | AllocS e v σ l :
@@ -306,7 +315,7 @@ Lemma atomic_head_step e1 σ1 e2 σ2 ef :
   atomic e1 → head_step e1 σ1 e2 σ2 ef → is_Some (to_val e2).
 Proof.
   destruct 2; simpl; rewrite ?to_of_val; try by eauto.
-  repeat (case_match || contradiction || simplify_eq/=); eauto.
+  unfold subst'; repeat (case_match || contradiction || simplify_eq/=); eauto.
 Qed.
 
 Lemma atomic_step e1 σ1 e2 σ2 ef :
@@ -351,9 +360,6 @@ Lemma alloc_fresh e v σ :
   let l := fresh (dom _ σ) in
   to_val e = Some v → head_step (Alloc e) σ (Loc l) (<[l:=v]>σ) None.
 Proof. by intros; apply AllocS, (not_elem_of_dom (D:=gset _)), is_fresh. Qed.
-
-Lemma subst_empty e v : subst e "" v = e.
-Proof. induction e; simpl; repeat case_decide; intuition auto with f_equal. Qed.
 End heap_lang.
 
 (** Language *)
