barrier/barrier.v
@@ -1,6 +1,6 @@
 From heap_lang Require Export substitution notation.
 
-Definition newbarrier : val := λ: "", ref #0.
+Definition newbarrier : val := λ: <>, ref #0.
 Definition signal : val := λ: "x", "x" <- #1.
 Definition wait : val :=
   rec: "wait" "x" := if: !"x" = #1 then #() else "wait" "x".
