heap_lang/derived.v
@@ -2,12 +2,12 @@ From heap_lang Require Export lifting.
 Import uPred.
 
 (** Define some derived forms, and derived lemmas about them. *)
-Notation Lam x e := (Rec "" x e).
+Notation Lam x e := (Rec BAnom x e).
 Notation Let x e1 e2 := (App (Lam x e2) e1).
-Notation Seq e1 e2 := (Let "" e1 e2).
-Notation LamV x e := (RecV "" x e).
+Notation Seq e1 e2 := (Let BAnom e1 e2).
+Notation LamV x e := (RecV BAnom x e).
 Notation LetCtx x e2 := (AppRCtx (LamV x e2)).
-Notation SeqCtx e2 := (LetCtx "" e2).
+Notation SeqCtx e2 := (LetCtx BAnom e2).
 Notation Skip := (Seq (Lit LitUnit) (Lit LitUnit)).
 
 Section derived.
@@ -18,18 +18,18 @@ Implicit Types Φ : val → iProp heap_lang Σ.
 (** Proof rules for the sugar *)
 Lemma wp_lam E x ef e v Φ :
   to_val e = Some v →
-  ▷ || subst ef x v @ E {{ Φ }} ⊑ || App (Lam x ef) e @ E {{ Φ }}.
-Proof. intros. by rewrite -wp_rec ?subst_empty. Qed.
+  ▷ || subst' ef x v @ E {{ Φ }} ⊑ || App (Lam x ef) e @ E {{ Φ }}.
+Proof. intros. by rewrite -wp_rec. Qed.
 
 Lemma wp_let E x e1 e2 v Φ :
   to_val e1 = Some v →
-  ▷ || subst e2 x v @ E {{ Φ }} ⊑ || Let x e1 e2 @ E {{ Φ }}.
+  ▷ || subst' e2 x v @ E {{ Φ }} ⊑ || Let x e1 e2 @ E {{ Φ }}.
 Proof. apply wp_lam. Qed.
 
 Lemma wp_seq E e1 e2 v Φ :
   to_val e1 = Some v →
   ▷ || e2 @ E {{ Φ }} ⊑ || Seq e1 e2 @ E {{ Φ }}.
-Proof. intros ?. rewrite -wp_let // subst_empty //. Qed.
+Proof. intros ?. by rewrite -wp_let. Qed.
 
 Lemma wp_skip E Φ : ▷ Φ (LitV LitUnit) ⊑ || Skip @ E {{ Φ }}.
 Proof. rewrite -wp_seq // -wp_value //. Qed.
